BoogieLang/Lang.thy
@@ -38,6 +38,7 @@ datatype expr
   | UnOp unop "expr"
   | BinOp "(expr)" binop "(expr)" ("_ \<guillemotleft>_\<guillemotright> _" [80,0,81] 80) 
   | FunExp fname "ty list" "(expr list)" (* second argument: type instantiation *)
+  | MapSelect "expr" "expr"
   | CondExp expr expr expr
   | Old expr
 (* value quantification *)
